merging main

pulse/src/ocaml/plugin/generated/Pulse_Syntax_Pure.ml
@@ -328,7 +328,8 @@ let (is_arrow :
   fun t ->
     match t.Pulse_Syntax_Base.t with
     | Pulse_Syntax_Base.Tm_FStar host_term ->
-        (match FStar_Reflection_V2_Builtins.inspect_ln host_term with
+        (match FStar_Reflection_V2_Derived.inspect_ln_unascribe host_term
+         with
          | FStar_Reflection_V2_Data.Tv_Arrow (b, c) ->
              let uu___ = FStar_Reflection_V2_Builtins.inspect_binder b in
              (match uu___ with
@@ -365,6 +366,34 @@ let (is_arrow :
                                                 (FStar_Reflection_V2_Builtins.range_of_term
                                                    host_term))
                                          }, q, c1)))
+                        | FStar_Reflection_V2_Data.C_Eff
+                            (uu___3, eff_name, result, uu___4, uu___5) ->
+                            if eff_name = ["Prims"; "Tot"]
+                            then
+                              op_let_Question
+                                (Pulse_Readback.readback_ty sort)
+                                (fun binder_ty ->
+                                   op_let_Question
+                                     (match Pulse_Readback.readback_comp
+                                              result
+                                      with
+                                      | FStar_Pervasives_Native.Some c1 ->
+                                          FStar_Pervasives_Native.Some c1
+                                      | FStar_Pervasives_Native.None ->
+                                          FStar_Pervasives_Native.None)
+                                     (fun c1 ->
+                                        FStar_Pervasives_Native.Some
+                                          ({
+                                             Pulse_Syntax_Base.binder_ty =
+                                               binder_ty;
+                                             Pulse_Syntax_Base.binder_ppname
+                                               =
+                                               (Pulse_Syntax_Base.mk_ppname
+                                                  ppname
+                                                  (FStar_Reflection_V2_Builtins.range_of_term
+                                                     host_term))
+                                           }, q, c1)))
+                            else FStar_Pervasives_Native.None
                         | uu___3 -> FStar_Pervasives_Native.None)))
          | uu___ -> FStar_Pervasives_Native.None)
     | uu___ -> FStar_Pervasives_Native.None
