pulse/share/steel/examples/pulse/CustomSyntax.fst
@@ -14,8 +14,8 @@ fn unfold_test (r:ref U32.t)
   requires folded_pts_to r 'n
   ensures folded_pts_to r 'n
 {
-  with n. unfold (folded_pts_to r n);
-  with n. fold (folded_pts_to r n)
+  unfold folded_pts_to;
+  fold folded_pts_to
 }
 ```
 
