pulse/src/syntax_extension/header.sh
@@ -1,0 +1,9 @@
+#!/bin/bash
+
+header=`cat header.txt`
+
+for file in `find ./ -iname "*.fst"`
+do
+  echo "adding header to $file"
+  sed -i -e "1i $header" $file
+done
